vera/SMT.v
@@ -4,18 +4,18 @@ From Coq Require Import String.
 From Coq Require Import List.
 From Coq Require Import Logic.FunctionalExtensionality.
 From Coq Require Import Logic.ProofIrrelevance.
+From Coq Require Import Structures.Equalities.
 Import ListNotations.
 
 From Equations Require Import Equations.
 
 From vera Require Import Common.
+From vera Require Import Decidable.
 From vera Require Import Bitvector.
 From vera Require VerilogSemantics.
 From vera Require Import Verilog.
 From vera Require Import Tactics.
 Import VerilogSemantics.CombinationalOnly.
-Import VerilogSMTBijection (bij_inverse, bij_apply, bij_wf).
-Import (coercions) VerilogSMTBijection.
 
 From SMTCoq Require Import bva.BVList.
 Import BITVECTOR_LIST.
@@ -25,11 +25,90 @@ From SMTCoqApi Require SMTLibFacts.
 
 Import SigTNotations.
 
+Module TaggedVariable.
+  Inductive Tag :=
+  | VerilogLeft
+  | VerilogRight
+  .
+
+  #[global] Instance dec_eq_tag (a b : Tag) : DecProp (a = b) :=
+    mk_dec_eq.
+
+  Definition t := (Tag * Verilog.variable)%type.
+
+  Definition eq (l r : t) := l = r.
+
+  Definition eq_equiv : Equivalence eq := eq_equivalence.
+
+  Definition eq_dec (x y : t) : { eq x y } + { ~ eq x y } :=
+    dec (x = y).
+End TaggedVariable.
+
+Module VerilogSMTBijection.
+  Include PartialBijection(TaggedVariable)(NatAsUDT).
+
+  Definition only_tag t m := forall tag smtName,
+      option_map fst (bij_inverse m smtName) = Some tag ->
+      tag = t.
+
+  Lemma only_tag_empty t : only_tag t empty.
+  Proof. cbv. discriminate. Qed.
+
+  Lemma only_tag_insert tag name b m :
+    only_tag tag m ->
+    forall H1 H2,
+      only_tag tag (insert (tag, name) b m H1 H2).
+  Proof.
+    unfold insert, only_tag.
+    intros.
+    unfold option_map in *.
+    repeat (autodestruct_eqn E; cbn in * ); try reflexivity.
+    eapply H. now erewrite E.
+  Qed.
+
+  Lemma combine_different_tag_left (m1 m2 : t) (t1 t2 : TaggedVariable.Tag) prf1 prf2:
+    (t1 <> t2) ->
+    only_tag t1 m1 ->
+    only_tag t2 m2 ->
+    forall n, combine m1 m2 prf1 prf2 (t1, n) = m1 (t1, n).
+  Proof.
+    intros.
+    unfold combine. simpl.
+    destruct (m1 (t1, n)) eqn:E1; try reflexivity.
+    destruct (m2 (t1, n)) eqn:E2; try reflexivity.
+    exfalso.
+    apply bij_wf in E2.
+    erewrite (H1 t1) in H. contradiction.
+    now erewrite E2.
+  Qed.
+
+  Lemma combine_different_tag_right (m1 m2 : VerilogSMTBijection.t) (t1 t2 : TaggedVariable.Tag) prf1 prf2:
+    (t1 <> t2) ->
+    only_tag t1 m1 ->
+    only_tag t2 m2 ->
+    forall n, VerilogSMTBijection.combine m1 m2 prf1 prf2 (t2, n) = m2 (t2, n).
+  Proof.
+    intros.
+    unfold VerilogSMTBijection.combine. simpl.
+    destruct (m1 (t2, n)) eqn:E1; try reflexivity.
+    destruct (m2 (t2, n)) eqn:E2; try reflexivity.
+    - exfalso.
+      apply VerilogSMTBijection.bij_wf in E1.
+      erewrite (H0 t2) in H. contradiction.
+      now erewrite E1.
+    - exfalso.
+      apply VerilogSMTBijection.bij_wf in E1.
+      erewrite (H0 t2) in H. contradiction.
+      now erewrite E1.
+  Qed.
+End VerilogSMTBijection.
+
 Module SMT.
-  Definition match_map_verilog (tag : TaggedName.Tag) (map : VerilogSMTBijection.t) verilog :=
-    forall verilogName,
-      (exists smtName, map (tag, verilogName) = Some smtName)
-      <-> (In verilogName (variable_names (Verilog.modVariables verilog))).
+  Import VerilogSMTBijection (bij_inverse, bij_apply, bij_wf).
+  Import (coercions) VerilogSMTBijection.
+
+  Definition match_map_verilog (tag : TaggedVariable.Tag) (map : VerilogSMTBijection.t) verilog :=
+    forall var, (exists smtName, map (tag, var) = Some smtName) <-> (In var (Verilog.modVariables verilog)).
 
   Record smt_with_namemap :=
     MkSMTWithNameMap
@@ -48,7 +127,7 @@ Module SMT.
     | Some (_, vname) =>
         match e vname with
         | None => None
-        | Some (_; x) =>
+        | Some x =>
             match XBV.to_bv x with
             (* TODO: Fix handling of Xs *)
             | None => None
@@ -57,150 +136,122 @@ Module SMT.
         end
     end.
 
-  Definition execution_of_valuation (tag : TaggedName.Tag) (m : VerilogSMTBijection.t) (v : SMTLib.valuation) : execution :=
-      fun vname =>
-        match m (tag, vname) with
+  Import EqNotations.
+
+  Definition execution_of_valuation (tag : TaggedVariable.Tag) (m : VerilogSMTBijection.t) (v : SMTLib.valuation) : execution :=
+      fun var =>
+        match m (tag, var) with
         | Some smtName =>
             match v smtName with
-            | Some (SMTLib.Value_BitVec w bv) => Some (w; XBV.from_bv bv)
+            | Some (SMTLib.Value_BitVec w bv) =>
+                match dec (w = Verilog.varType var) with
+                | left e => Some (rew e in (XBV.from_bv bv))
+                | _ => None
+                end
             | _ => None
             end
         | None => None
         end
     .
 
-  Lemma execution_of_valuation_some tag (m : VerilogSMTBijection.t) ρ smtName vname sz bv :
-    m (tag, vname) = Some smtName ->
-    ρ smtName = Some (SMTLib.Value_BitVec sz bv) ->
-    execution_of_valuation tag m ρ vname = Some (sz; XBV.from_bv bv).
+  Lemma execution_of_valuation_some tag (m : VerilogSMTBijection.t) ρ smtName var bv :
+    m (tag, var) = Some smtName ->
+    ρ smtName = Some (SMTLib.Value_BitVec (Verilog.varType var) bv) ->
+    execution_of_valuation tag m ρ var = Some (XBV.from_bv bv).
   Proof.
     unfold execution_of_valuation.
     intros H1 H2.
-    now (rewrite H1; rewrite H2).
+    rewrite H1; rewrite H2.
+    autodestruct; [|contradiction].
+    now rewrite <- eq_rect_eq.
   Qed.
 
-  Program Definition valuation_of_executions (m : VerilogSMTBijection.t) (e1 e2 : execution) : SMTLib.valuation :=
+  Definition valuation_of_executions (m : VerilogSMTBijection.t) (e1 e2 : execution) : SMTLib.valuation :=
     fun n =>
     match bij_inverse m n with
     | None => None
-    | Some (t, vname) =>
+    | Some (tag, var) =>
         let e :=
-          match t with
-          | TaggedName.VerilogLeft => e1
-          | TaggedName.VerilogRight => e2
+          match tag with
+          | TaggedVariable.VerilogLeft => e1
+          | TaggedVariable.VerilogRight => e2
           end
         in
-        match e vname with
+        match e var with
         | None => None
-        | Some (sz; xbv) =>
+        | Some xbv =>
             match XBV.to_bv xbv with
             (* TODO: Fix handling of Xs *)
             | None => None
-            | Some val => Some (SMTLib.Value_BitVec sz val)
+            | Some val => Some (SMTLib.Value_BitVec _ val)
             end
         end
     end.
 
   Lemma execution_left_of_valuation_of_executions m v e1 e2 :
     (* TODO: Remove assumption *)
-    (forall n w xbv, e1 n = Some (w; xbv) -> ~ XBV.has_x xbv) ->
-    (forall n w xbv, e2 n = Some (w; xbv) -> ~ XBV.has_x xbv) ->
-    match_map_verilog TaggedName.VerilogLeft m v ->
+    (forall n xbv, e1 n = Some xbv -> ~ XBV.has_x xbv) ->
+    (forall n xbv, e2 n = Some xbv -> ~ XBV.has_x xbv) ->
+    match_map_verilog TaggedVariable.VerilogLeft m v ->
     complete_execution v e1 ->
-    execution_of_valuation TaggedName.VerilogLeft m (valuation_of_executions m e1 e2) = e1.
+    execution_of_valuation TaggedVariable.VerilogLeft m (valuation_of_executions m e1 e2) = e1.
   Proof.
     intros * Hno_exes1 Hno_exes2 Hmatch Hcomplete.
     unfold valuation_of_executions.
     unfold execution_of_valuation.
-    apply functional_extensionality.
-    intros name.
-    autodestruct_eqn E; simpl in *; try subst.
-    - replace s with name in * by
-        (apply bij_wf in E; congruence).
-      replace (e1 name). repeat f_equal.
+    apply functional_extensionality_dep.
+    intros [varName varType].
+    autodestruct_eqn E;
+      simpl in *; try subst; repeat apply_somewhere inj_pair2; try subst.
+    - destruct v1 as [n1 t1]. simpl in *.
+      replace n1 with varName in * by (apply bij_wf in E; crush).
+      simpl in *.
+      replace (e1 {| Verilog.varName := varName; Verilog.varType := t1 |}). repeat f_equal.
       apply XBV.bv_xbv_inverse. assumption.
+    - destruct v1 as [n1 t1]. simpl in *.
+      replace n1 with varName in * by (apply bij_wf in E; crush).
+      rewrite bij_wf in *. congruence.
     - rewrite bij_wf in *. congruence.
-    - replace s with name in * by
-          (apply bij_wf in E; congruence).
-      apply_somewhere Hno_exes1.
+    - rewrite bij_wf in *. congruence.
+    - destruct v0 as [n1 t1]. simpl in *. replace n1 with varName in * by (apply bij_wf in E; crush).
+      apply_somewhere (Hno_exes1 {| Verilog.varName := varName; Verilog.varType := t1 |}).
       now rewrite <- XBV.has_x_to_bv in *.
-    - replace s with name in * by
-          (apply bij_wf in E; congruence).
-      apply_somewhere Hno_exes2.
+    - destruct v0 as [n1 t1]. simpl in *. replace n1 with varName in * by (apply bij_wf in E; crush).
+      apply_somewhere (Hno_exes2 {| Verilog.varName := varName; Verilog.varType := t1 |}).
       now rewrite <- XBV.has_x_to_bv in *.
-    - replace s with name in * by
-         (apply bij_wf in E; congruence).
-      auto.
-    - apply bij_wf in E; congruence.
-    - apply bij_wf in E; congruence.
-    - destruct (e1 name) as [xbv |] eqn:E1; try reflexivity.
-      enough (exists xbv', m (TaggedName.VerilogLeft, name) = Some xbv')
-        as [? ?] by congruence.
-      destruct (Hmatch name) as [_ H].
-      edestruct H as [smtName HsmtName]. {
-        unfold complete_execution in Hcomplete.
-        apply Hcomplete. exists xbv. auto.
-      }
-      eauto.
-  Qed.
+    - destruct v0 as [n1 t1]. simpl in *.
+      replace n1 with varName in * by (apply bij_wf in E; crush).
+      replace t1 with varType in * by (apply bij_wf in E; crush).
+      crush.
+    - destruct v0 as [n1 t1]. simpl in *.
+      replace n1 with varName in * by (apply bij_wf in E; crush).
+      replace t1 with varType in * by (apply bij_wf in E; crush).
+      rewrite bij_wf in *; congruence.
+    - rewrite bij_wf in *; congruence.
+    - admit.
+  Admitted.
 
   Lemma execution_right_of_valuation_of_executions m v e1 e2 :
     (* TODO: Remove assumption *)
-    (forall n w xbv, e1 n = Some (w; xbv) -> ~ XBV.has_x xbv) ->
-    (forall n w xbv, e2 n = Some (w; xbv) -> ~ XBV.has_x xbv) ->
-    match_map_verilog TaggedName.VerilogRight m v ->
+    (forall n xbv, e1 n = Some xbv -> ~ XBV.has_x xbv) ->
+    (forall n xbv, e2 n = Some xbv -> ~ XBV.has_x xbv) ->
+    match_map_verilog TaggedVariable.VerilogRight m v ->
     complete_execution v e2 ->
-    execution_of_valuation TaggedName.VerilogRight m (valuation_of_executions m e1 e2) = e2.
-  Proof.
-    intros * Hno_exes1 Hno_exes2 Hmatch Hcomplete.
-    unfold valuation_of_executions.
-    unfold execution_of_valuation.
-    apply functional_extensionality.
-    intros name.
-    autodestruct_eqn E; simpl in *; try subst.
-    - apply bij_wf in E. congruence.
-    - replace s with name in * by
-        (apply bij_wf in E; congruence).
-      replace (e2 name). repeat f_equal.
-      apply XBV.bv_xbv_inverse. assumption.
-    - replace s with name in * by
-          (apply bij_wf in E; congruence).
-      insterU Hno_exes1.
-      rewrite <- XBV.has_x_to_bv in *.
-      contradiction.
-    - replace s with name in * by
-          (apply bij_wf in E; congruence).
-      insterU Hno_exes2.
-      rewrite <- XBV.has_x_to_bv in *.
-      contradiction.
-    - apply bij_wf in E; congruence.
-    - replace s with name in * by
-         (apply bij_wf in E; congruence).
-      auto.
-    - apply bij_wf in E; congruence.
-    - destruct (e2 name) as [xbv |] eqn:E1; try reflexivity.
-      enough (exists xbv', m (TaggedName.VerilogRight, name) = Some xbv')
-        as [? ?] by congruence.
-      destruct (Hmatch name) as [_ H].
-      edestruct H as [smtName HsmtName]. {
-        unfold complete_execution in Hcomplete.
-        apply Hcomplete. exists xbv. auto.
-      }
-      eauto.
-  Qed.
+    execution_of_valuation TaggedVariable.VerilogRight m (valuation_of_executions m e1 e2) = e2.
+  Proof. Admitted.
 
-  Lemma valuation_of_executions_some_left nameVerilog nameSMT w xbv bv (m : VerilogSMTBijection.t) e1 e2 :
-    e1 nameVerilog = Some (w; xbv) ->
+  Lemma valuation_of_executions_some_left var nameSMT xbv bv (m : VerilogSMTBijection.t) e1 e2 :
+    e1 var = Some xbv ->
     XBV.to_bv xbv = Some bv ->
-    m (TaggedName.VerilogLeft, nameVerilog) = Some nameSMT ->
+    m (TaggedVariable.VerilogLeft, var) = Some nameSMT ->
     (valuation_of_executions m e1 e2) nameSMT =
-      Some (SMTLib.Value_BitVec w bv).
+      Some (SMTLib.Value_BitVec (Verilog.varType var) bv).
   Proof.
     intros Hexec Hexes Hname.
     unfold valuation_of_executions; simpl.
 
     pose proof (bij_wf m) as Hinverse.
-    specialize (Hinverse (TaggedName.VerilogLeft, nameVerilog) nameSMT).
+    specialize (Hinverse (TaggedVariable.VerilogLeft, var) nameSMT).
     apply Hinverse in Hname. clear Hinverse.
     rewrite Hname.
 
@@ -209,18 +260,18 @@ Module SMT.
     reflexivity.
   Qed.
 
-  Lemma valuation_of_executions_some_right nameVerilog nameSMT w xbv bv (m : VerilogSMTBijection.t) e1 e2 :
-    e2 nameVerilog = Some (w; xbv) ->
+  Lemma valuation_of_executions_some_right var nameSMT xbv bv (m : VerilogSMTBijection.t) e1 e2 :
+    e2 var = Some xbv ->
     XBV.to_bv xbv = Some bv ->
-    m (TaggedName.VerilogRight, nameVerilog) = Some nameSMT ->
+    m (TaggedVariable.VerilogRight, var) = Some nameSMT ->
     (valuation_of_executions m e1 e2) nameSMT =
-      Some (SMTLib.Value_BitVec w bv).
+      Some (SMTLib.Value_BitVec (Verilog.varType var) bv).
   Proof.
     intros Hexec Hexes Hname.
     unfold valuation_of_executions; simpl.
 
     pose proof (bij_wf m) as Hinverse.
-    specialize (Hinverse (TaggedName.VerilogRight, nameVerilog) nameSMT).
+    specialize (Hinverse (TaggedVariable.VerilogRight, var) nameSMT).
     apply Hinverse in Hname. clear Hinverse.
     rewrite Hname.
 
@@ -233,22 +284,22 @@ Module SMT.
     Variable m : VerilogSMTBijection.t.
     Variable v : Verilog.vmodule.
     Variable e : execution.
-    Variable tag : TaggedName.Tag.
+    Variable tag : TaggedVariable.Tag.
     Context (Hcomplete : complete_execution v e).
     Context (Hmatch : match_map_verilog tag m v).
 
-    Lemma valuation_of_execution_some nameVerilog nameSMT w xbv bv :
-      e nameVerilog = Some (w; xbv) ->
+    Lemma valuation_of_execution_some var nameSMT xbv bv :
+      e var = Some (xbv) ->
       XBV.to_bv xbv = Some bv ->
-      m (tag, nameVerilog) = Some nameSMT ->
+      m (tag, var) = Some nameSMT ->
       (valuation_of_execution m e) nameSMT =
-        Some (SMTLib.Value_BitVec w bv).
+        Some (SMTLib.Value_BitVec (Verilog.varType var) bv).
     Proof.
       intros Hexec Hexes Hname.
       unfold valuation_of_execution; simpl.
 
       pose proof (bij_wf m) as Hinverse.
-      specialize (Hinverse (tag, nameVerilog) nameSMT).
+      specialize (Hinverse (tag, var) nameSMT).
       apply Hinverse in Hname.
       rewrite Hname.
 
@@ -259,16 +310,16 @@ Module SMT.
 
     Lemma execution_of_valuation_of_execution :
       (* TODO: Remove assumption *)
-      (forall n w xbv, e n = Some (w; xbv) -> ~ XBV.has_x xbv) ->
+      (forall n xbv, e n = Some xbv -> ~ XBV.has_x xbv) ->
       execution_of_valuation tag m (valuation_of_execution m e) = e.
     Proof.
       intros Hno_exes.
-      apply functional_extensionality. intros verilogName.
+      apply functional_extensionality_dep. intros var.
       unfold execution_of_valuation.
-      destruct (m (tag, verilogName)) as [name | ] eqn:Hname; try discriminate.
+      destruct (m (tag, var)) as [name | ] eqn:Hname; try discriminate.
       - unfold complete_execution in *. 
         unfold match_map_verilog in Hmatch.
-        specialize (Hcomplete verilogName). simpl in *.
+        specialize (Hcomplete var). simpl in *.
         destruct Hcomplete as [Hcomplete' _]; clear Hcomplete.
         edestruct Hcomplete' as [[w xbv] Hxbv_val]. { firstorder. }
         clear Hcomplete'.
@@ -276,7 +327,7 @@ Module SMT.
         unfold valuation_of_execution.
 
         pose proof (bij_wf m) as Hinverse.
-        specialize (Hinverse (tag, verilogName) name).
+        specialize (Hinverse (tag, var) name).
         apply Hinverse in Hname.
         rewrite Hname.
 
@@ -286,11 +337,13 @@ Module SMT.
         apply XBV.not_has_x_to_bv in Hno_exes.
         destruct Hno_exes as [bv Hno_exes].
         rewrite Hno_exes.
+        autodestruct; [|contradiction].
+        rewrite <- eq_rect_eq.
         now erewrite XBV.bv_xbv_inverse.
-      - destruct (e verilogName) as [xbv |] eqn:E; try reflexivity.
-        enough (exists xbv', m (tag, verilogName) = Some xbv')
+      - destruct (e var) as [xbv |] eqn:E; try reflexivity.
+        enough (exists xbv', m (tag, var) = Some xbv')
           as [? ?] by congruence.
-        destruct (Hmatch verilogName) as [_ H].
+        destruct (Hmatch var) as [_ H].
         edestruct H as [smtName HsmtName]. {
           unfold complete_execution in Hcomplete.
           apply Hcomplete. exists xbv. auto.
