vera/VerilogEquivalence.v
@@ -37,7 +37,7 @@ Local Open Scope string.
 
 Equations mk_var_same (var : Verilog.variable) (namemap : VerilogSMTBijection.t)
   : sum string SMTLib.term := {
-  | var, namemap with namemap (TaggedName.VerilogLeft, Verilog.varName var), namemap (TaggedName.VerilogRight, Verilog.varName var) => {
+  | var, namemap with namemap (TaggedVariable.VerilogLeft, Verilog.varName var), namemap (TaggedVariable.VerilogRight, Verilog.varName var) => {
     | Some smt_name1, Some smt_name2 =>
         inr (SMTLib.Term_Eq (SMTLib.Term_Const smt_name1) (SMTLib.Term_Const smt_name2))
     | _, _ => inl "mk_var_same"%string
@@ -61,7 +61,7 @@ Equations mk_inputs_same (inputs : list Verilog.variable) (namemap : VerilogSMTB
 
 Equations mk_var_distinct (var : Verilog.variable) (namemap : VerilogSMTBijection.t)
   : sum string SMTLib.term := {
-  | var, namemap with namemap (TaggedName.VerilogLeft, Verilog.varName var), namemap (TaggedName.VerilogRight, Verilog.varName var) => {
+  | var, namemap with namemap (TaggedVariable.VerilogLeft, Verilog.varName var), namemap (TaggedVariable.VerilogRight, Verilog.varName var) => {
     | Some smt_name1, Some smt_name2 =>
         inr (SMTLib.Term_Not (SMTLib.Term_Eq (SMTLib.Term_Const smt_name1) (SMTLib.Term_Const smt_name2)))
     | _, _ => inl "mk_var_distinct"%string
@@ -90,8 +90,8 @@ Program Definition equivalence_query_canonical
   inputs_ok1 <- assert_dec (Verilog.module_inputs canonical_verilog1 = Verilog.module_inputs canonical_verilog2) "Inputs don't match" ;;
   outputs_ok1 <- assert_dec (Verilog.module_outputs canonical_verilog1 = Verilog.module_outputs canonical_verilog2) "Outputs don't match" ;;
 
-  smt1 <- VerilogToSMT.verilog_to_smt TaggedName.VerilogLeft 0 canonical_verilog1 ;;
-  smt2 <- VerilogToSMT.verilog_to_smt TaggedName.VerilogRight (1 + SMT.max_var (SMT.query smt1)) canonical_verilog2 ;;
+  smt1 <- VerilogToSMT.verilog_to_smt TaggedVariable.VerilogLeft 0 canonical_verilog1 ;;
+  smt2 <- VerilogToSMT.verilog_to_smt TaggedVariable.VerilogRight (1 + SMT.max_var (SMT.query smt1)) canonical_verilog2 ;;
 
   let nameMap := VerilogSMTBijection.combine (SMT.nameMap smt1) (SMT.nameMap smt2) _ _ in
 
